common/SimMemInj.v
@@ -1,0 +1,611 @@
+Require Import Coqlib.
+Require Import Memory.
+Require Import Values.
+Require Import Maps.
+Require Import Events.
+Require Import Globalenvs.
+Require Import AST.
+Require Import sflib.
+Require Import RelationClasses.
+From Paco Require Import paco.
+
+Require Import Integers Linking.
+
+Set Implicit Arguments.
+
+Hint Extern 998 => xomega : xomega.
+Hint Extern 999 => congruence : congruence.
+
+Definition less1 X0 (p q: X0 -> Prop) := (forall x0 (PR: p x0 : Prop), q x0 : Prop).
+Definition less2 X0 X1 (p q: X0 -> X1 -> Prop) := (forall x0 x1 (PR: p x0 x1 : Prop), q x0 x1 : Prop).
+Definition less3 X0 X1 X2 (p q: X0 -> X1 -> X2 -> Prop) := (forall x0 x1 x2 (PR: p x0 x1 x2 : Prop), q x0 x1 x2 : Prop).
+Definition less4 X0 X1 X2 X3 (p q: X0 -> X1 -> X2 -> X3 -> Prop) := (forall x0 x1 x2 x3 (PR: p x0 x1 x2 x3 : Prop), q x0 x1 x2 x3 : Prop).
+
+Notation "p <1= q" := (less1 p q) (at level 50).
+Notation "p <2= q" := (less2 p q) (at level 50).
+Notation "p <3= q" := (less3 p q) (at level 50).
+Notation "p <4= q" := (less4 p q) (at level 50).
+
+Global Program Instance less1_PreOrder X0: PreOrder (@less1 X0).
+Next Obligation. ii. ss. Qed.
+Next Obligation. ii. eapply H0; eauto. Qed.
+Global Program Instance less2_PreOrder X0 X1: PreOrder (@less2 X0 X1).
+Next Obligation. ii. ss. Qed.
+Next Obligation. ii. eapply H0; eauto. Qed.
+Global Program Instance less3_PreOrder X0 X1 X2: PreOrder (@less3 X0 X1 X2).
+Next Obligation. ii. ss. Qed.
+Next Obligation. ii. eapply H0; eauto. Qed.
+Global Program Instance less4_PreOrder X0 X1 X2 X3 : PreOrder (@less4 X0 X1 X2 X3).
+Next Obligation. ii. ss. Qed.
+Next Obligation. ii. eapply H0; eauto. Qed.
+Hint Unfold less1 less2 less3 less4.
+
+
+(* Copied from CRELLVM *)
+Inductive frozen (f_old f_new: meminj) (bound_src bound_tgt: block): Prop :=
+| frozen_intro
+    (NEW_IMPLIES_OUTSIDE:
+       forall b_src b_tgt delta
+              (NEW: f_old b_src = None /\ f_new b_src = Some(b_tgt, delta)),
+         <<OUTSIDE_SRC: (bound_src <= b_src)%positive>> /\ <<OUTSIDE_TGT: (bound_tgt <= b_tgt)%positive>>)
+.
+
+Remark inject_separated_frozen
+       f_old f_new m_src m_tgt
+  :
+    Events.inject_separated f_old f_new m_src m_tgt <->
+    frozen f_old f_new m_src.(Mem.nextblock) m_tgt.(Mem.nextblock)
+.
+Proof.
+  unfold Events.inject_separated in *.
+  unfold Mem.valid_block in *.
+  split; i.
+  - econs; eauto.
+    i. des.
+    hexploit H; eauto. i; des.
+    splits; xomega.
+  - inv H.
+    exploit NEW_IMPLIES_OUTSIDE; eauto.
+    i; des.
+    split; xomega.
+Qed.
+
+Lemma frozen_preserves_src
+      f_old f_new
+      (INJECT: inject_incr f_old f_new)
+      bound_src bound_tgt
+      (FROZEN: frozen f_old f_new bound_src bound_tgt)
+      b_src
+      (INSIDE: (b_src < bound_src)%positive)
+  :
+    <<PRESERVED: f_old b_src = f_new b_src>>
+.
+Proof.
+  inv FROZEN.
+  destruct (f_old b_src) eqn:T0; ss;
+    destruct (f_new b_src) eqn:T1; ss.
+  - destruct p, p0; ss.
+    exploit INJECT; eauto; []; i; des.
+    clarify.
+  - destruct p; ss.
+    exploit INJECT; eauto; []; i; des.
+    clarify.
+  - destruct p; ss.
+    exploit NEW_IMPLIES_OUTSIDE; eauto; []; i; des.
+    exfalso.
+    xomega.
+Qed.
+
+Lemma frozen_preserves_tgt
+      f_old f_new
+      (INJECT: inject_incr f_old f_new)
+      bound_src bound_tgt
+      (FROZEN: frozen f_old f_new bound_src bound_tgt)
+      b_tgt
+      (INSIDE: (b_tgt < bound_tgt)%positive)
+  :
+    <<PRESERVED: forall b_src delta (NOW: f_new b_src = Some (b_tgt, delta)),
+      <<OLD: f_old b_src = Some (b_tgt, delta)>> >>
+.
+Proof.
+  inv FROZEN.
+  ii.
+  destruct (f_old b_src) eqn:T; ss.
+  - destruct p; ss.
+    exploit INJECT; eauto; []; i; des.
+    clarify.
+  - exfalso.
+    exploit NEW_IMPLIES_OUTSIDE; eauto; []; i; des.
+    xomega.
+Qed.
+
+Lemma frozen_shortened
+      f_old f_new
+      bd_src0 bd_tgt0
+      (FROZEN: frozen f_old f_new bd_src0 bd_tgt0)
+      bd_src1 bd_tgt1
+      (SHORT_SRC: (bd_src1 <= bd_src0)%positive)
+      (SHORT_TGT: (bd_tgt1 <= bd_tgt0)%positive)
+  :
+    <<FROZEN: frozen f_old f_new bd_src1 bd_tgt1>>
+.
+Proof.
+  inv FROZEN.
+  econs; eauto.
+  ii. des.
+  hexploit NEW_IMPLIES_OUTSIDE; eauto; []; i; des. clear NEW_IMPLIES_OUTSIDE.
+  split; ss.
+  - red. etransitivity; eauto.
+  - red. etransitivity; eauto.
+Qed.
+
+Lemma frozen_refl
+      f
+      bound_src bound_tgt
+  :
+    <<FROZEN: frozen f f bound_src bound_tgt>>
+.
+Proof.
+  econs; eauto. i; des. clarify.
+Qed.
+
+Lemma loc_unmapped_frozen
+      F F'
+      fbound_src fbound_tgt
+      (FROZEN : frozen F F' fbound_src fbound_tgt)
+      b ofs
+      (BOUND: Plt b fbound_src)
+      (UNMAPPED: loc_unmapped F b ofs)
+  :
+    loc_unmapped F' b ofs
+.
+Proof.
+  unfold loc_unmapped in *.
+  destruct (F' b) eqn:T; ss.
+  destruct p; ss.
+  inv FROZEN.
+  exploit NEW_IMPLIES_OUTSIDE; eauto.
+  i; des. xomega.
+Qed.
+
+Lemma loc_out_of_reach_frozen
+      F F'
+      fbound_src fbound_tgt
+      (INCR: inject_incr F F')
+      (FROZEN : frozen F F' fbound_src fbound_tgt)
+      b ofs
+      (BOUND: Plt b fbound_tgt)
+      m0 m1
+      (UNMAPPED: loc_out_of_reach F m0 b ofs)
+      (MAXPERM: forall b0 delta (MAPPED: F b0 = Some (b, delta)),
+          Mem.perm m1 b0 (ofs - delta) Max Nonempty -> Mem.perm m0 b0 (ofs - delta) Max Nonempty)
+  :
+    loc_out_of_reach F' m1 b ofs
+.
+Proof.
+  unfold loc_out_of_reach in *.
+  i.
+  exploit frozen_preserves_tgt; eauto.
+  i. des.
+  hexploit UNMAPPED; eauto.
+Qed.
+
+
+Section MEMINJ.
+
+(* Local Existing Instance Val.mi_normal. *)
+(* Variable gbound_src gbound_tgt: block. *)
+
+Record t' := mk {
+  src: mem;
+  tgt: mem;
+  inj: meminj;
+  src_external: block -> Z -> Prop;
+  tgt_external: block -> Z -> Prop;
+  src_parent_nb: block;
+  tgt_parent_nb: block;
+}.
+
+Definition valid_blocks (m: mem): block -> Z -> Prop := fun b _ => m.(Mem.valid_block) b.
+Hint Unfold valid_blocks.
+
+Definition src_private (sm: t'): block -> Z -> Prop :=
+  loc_unmapped sm.(inj) /2\ sm.(src).(valid_blocks)
+.
+
+Definition tgt_private (sm: t'): block -> Z -> Prop :=
+  loc_out_of_reach sm.(inj) sm.(src) /2\ sm.(tgt).(valid_blocks)
+.
+
+Hint Unfold src_private tgt_private.
+
+Inductive wf' (sm0: t'): Prop :=
+| wf_intro
+    (PUBLIC: Mem.inject sm0.(inj) sm0.(src) sm0.(tgt))
+    (SRCEXT: sm0.(src_external) <2= sm0.(src_private))
+    (TGTEXT: sm0.(tgt_external) <2= sm0.(tgt_private))
+    (SRCLE: (sm0.(src_parent_nb) <= sm0.(src).(Mem.nextblock))%positive)
+    (TGTLE: (sm0.(tgt_parent_nb) <= sm0.(tgt).(Mem.nextblock))%positive)
+.
+
+Inductive le' (mrel0 mrel1: t'): Prop :=
+| le_intro
+    (INCR: inject_incr mrel0.(inj) mrel1.(inj))
+    (SRCUNCHANGED: Mem.unchanged_on mrel0.(src_external) mrel0.(src) mrel1.(src))
+    (TGTUNCHANGED: Mem.unchanged_on mrel0.(tgt_external) mrel0.(tgt) mrel1.(tgt))
+    (SRCPARENTEQ: mrel0.(src_external) = mrel1.(src_external))
+    (SRCPARENTEQNB: mrel0.(src_parent_nb) = mrel1.(src_parent_nb))
+    (TGTPARENTEQ: mrel0.(tgt_external) = mrel1.(tgt_external))
+    (TGTPARENTEQNB: mrel0.(tgt_parent_nb) = mrel1.(tgt_parent_nb))
+    (FROZEN: frozen mrel0.(inj) mrel1.(inj) (mrel0.(src_parent_nb))
+                                            (mrel0.(tgt_parent_nb)))
+    (MAXSRC: forall
+        b ofs
+        (VALID: Mem.valid_block mrel0.(src) b)
+      ,
+        <<MAX: Mem.perm mrel1.(src) b ofs Max <1= Mem.perm mrel0.(src) b ofs Max>>)
+    (MAXTGT: forall
+        b ofs
+        (VALID: Mem.valid_block mrel0.(tgt) b)
+      ,
+        <<MAX: Mem.perm mrel1.(tgt) b ofs Max <1= Mem.perm mrel0.(tgt) b ofs Max>>)
+
+.
+
+Global Program Instance le'_PreOrder: RelationClasses.PreOrder le'.
+Next Obligation.
+  econs; eauto; try reflexivity; try apply Mem.unchanged_on_refl; eauto.
+  eapply frozen_refl; eauto.
+Qed.
+Next Obligation.
+  ii. inv H; inv H0.
+  des; clarify.
+  econs; eauto with mem congruence.
+  + eapply inject_incr_trans; eauto.
+  + eapply Mem.unchanged_on_trans; eauto with congruence.
+  + eapply Mem.unchanged_on_trans; eauto with congruence.
+  + econs; eauto.
+    ii; des.
+    destruct (inj y b_src) eqn:T.
+    * destruct p.
+      exploit INCR0; eauto. i; clarify.
+      inv FROZEN.
+      hexploit NEW_IMPLIES_OUTSIDE; eauto.
+    * inv FROZEN0.
+      hexploit NEW_IMPLIES_OUTSIDE; eauto; []; i; des.
+      split; ss; red; etransitivity; eauto.
+      { rewrite <- SRCPARENTEQNB. reflexivity. }
+      { rewrite <- TGTPARENTEQNB. reflexivity. }
+  + i. r. etransitivity.
+    { eapply MAXSRC0; eauto. eapply Plt_Ple_trans; eauto with mem.
+      eapply Mem.unchanged_on_nextblock; eauto. } (* added *)
+    eapply MAXSRC; eauto.
+  + i. r. etransitivity.
+    { eapply MAXTGT0; eauto. eapply Plt_Ple_trans; eauto with mem.
+      eapply Mem.unchanged_on_nextblock; eauto. } (* added *)
+    eapply MAXTGT; eauto.
+Qed.
+
+Definition lift' (mrel0: t'): t' :=
+  (mk mrel0.(src) mrel0.(tgt) mrel0.(inj)
+      mrel0.(src_private) mrel0.(tgt_private)
+      mrel0.(src).(Mem.nextblock) mrel0.(tgt).(Mem.nextblock))
+.
+
+Definition unlift' (mrel0 mrel1: t'): t' :=
+  (mk mrel1.(src) mrel1.(tgt) mrel1.(inj)
+      mrel0.(src_external) mrel0.(tgt_external)
+      mrel0.(src_parent_nb) mrel0.(tgt_parent_nb))
+.
+
+Lemma unlift_spec : forall mrel0 mrel1 : t',
+                  le' (lift' mrel0) mrel1 -> wf' mrel0 -> le' mrel0 (unlift' mrel0 mrel1).
+Proof.
+  i.
+  inv H; ss.
+  econs; ss; eauto; ii; des; ss.
+  - eapply Mem.unchanged_on_implies; eauto.
+    ii. eapply H0; eauto.
+  - eapply Mem.unchanged_on_implies; eauto.
+    ii. eapply H0; eauto.
+  - inv H0. ss.
+    eapply frozen_shortened; eauto.
+Qed.
+
+Lemma unlift_wf : forall mrel0 mrel1 : t',
+                wf' mrel0 ->
+                wf' mrel1 -> le' (lift' mrel0) mrel1 -> wf' (unlift' mrel0 mrel1).
+Proof.
+  i.
+  inv H. inv H0. inv H1.
+  des; clarify.
+  econs; ss; try etransitivity; eauto. (* eauto did well here *)
+  - (* etransitivity; eauto. *)
+    rewrite SRCPARENTEQ.
+    etransitivity; eauto.
+
+    (* u. bar. i; des. esplits; eauto. *)
+    (* + eapply loc_unmapped_frozen; eauto. *)
+    (* + unfold Mem.valid_block in *. xomega. *)
+  - (* etransitivity; eauto. *)
+    rewrite TGTPARENTEQ.
+    etransitivity; eauto.
+  - inv SRCUNCHANGED; ss.
+  - inv TGTUNCHANGED; ss.
+Qed.
+
+Lemma after_private_src
+      sm0 sm1
+      (FROZEN: frozen sm0.(inj) sm1.(inj) sm0.(src).(Mem.nextblock) sm0.(tgt).(Mem.nextblock))
+      (MLE: le' sm0.(lift') sm1)
+  :
+    sm0.(src_private) <2= sm1.(src_private)
+.
+Proof.
+  inv MLE. inv SRCUNCHANGED. ss.
+  unfold src_private, valid_blocks; ii; des; esplits; eauto.
+  - eapply loc_unmapped_frozen; eauto.
+  - unfold Mem.valid_block in *. xomega.
+Qed.
+
+Lemma after_private_tgt
+      sm0 sm1
+      (FROZEN: frozen sm0.(inj) sm1.(inj) sm0.(src).(Mem.nextblock) sm0.(tgt).(Mem.nextblock))
+      (MWF: wf' sm0)
+      (MLE: le' sm0.(lift') sm1)
+  :
+    sm0.(tgt_private) <2= sm1.(tgt_private)
+.
+Proof.
+  inv MLE. inv TGTUNCHANGED. ss.
+  unfold tgt_private, valid_blocks; ii; des; esplits; eauto.
+  - eapply loc_out_of_reach_frozen; eauto.
+    ii.
+    assert(VALID: Mem.valid_block (src sm0) b0).
+    { apply Classical_Prop.NNPP. ii. exploit Mem.mi_freeblocks; try apply MWF; eauto. ii. clarify. }
+    eapply MAXSRC; eauto.
+  - unfold Mem.valid_block in *. xomega.
+Qed.
+
+Section ORIGINALS.
+
+Lemma store_mapped
+      sm0 chunk v_src v_tgt blk_src ofs blk_tgt delta m_src0
+      (MWF: wf' sm0)
+      (STRSRC: Mem.store chunk sm0.(src) blk_src ofs v_src = Some m_src0)
+      (SIMBLK: sm0.(inj) blk_src = Some (blk_tgt, delta))
+      (SIMV: Val.inject sm0.(inj) v_src v_tgt)
+  :
+    exists sm1,
+      (<<MSRC: sm1.(src) = m_src0>>)
+      /\ (<<MINJ: sm1.(inj) = sm0.(inj)>>)
+      /\ (<<STRTGT: Mem.store chunk sm0.(tgt) blk_tgt (ofs + delta) v_tgt = Some sm1.(tgt)>>)
+      /\ (<<MWF: wf' sm1>>)
+      /\ (<<MLE: le' sm0 sm1>>)
+.
+Proof.
+  exploit Mem.store_mapped_inject; try apply MWF; eauto. i; des.
+  inv MWF.
+  eexists (mk _ _ _ _ _ _ _).
+  esplits; ss; eauto; cycle 1.
+  - econs; ss; eauto.
+    + eapply Mem.store_unchanged_on; eauto.
+      ii. apply SRCEXT in H2. red in H2. des. red in H2. clarify.
+    + eapply Mem.store_unchanged_on; eauto.
+      ii. apply TGTEXT in H2. red in H2. des. red in H2.
+      eapply H2; eauto. clear - STRSRC H1 H4.
+      apply Mem.store_valid_access_3 in STRSRC. destruct STRSRC.
+      eauto with mem xomega.
+    + eapply frozen_refl.
+    + ii. eapply Mem.perm_store_2; eauto.
+    + ii. eapply Mem.perm_store_2; eauto.
+  - econs; ss; eauto.
+    + etransitivity; eauto. unfold src_private. ss. ii; des. esplits; eauto.
+      unfold valid_blocks in *. eauto with mem.
+    + etransitivity; eauto. unfold tgt_private. ss. ii; des. esplits; eauto.
+      { ii. eapply PR. eauto with mem. eauto with mem. }
+      unfold valid_blocks in *. eauto with mem.
+    + etransitivity; eauto. erewrite <- Mem.nextblock_store; eauto. xomega.
+    + etransitivity; eauto. erewrite <- Mem.nextblock_store; eauto. xomega.
+Qed.
+
+Lemma storev_mapped
+      sm0 chunk v_src v_tgt addr_src addr_tgt m_src0
+      (MWF: wf' sm0)
+      (STRSRC: Mem.storev chunk sm0.(src) addr_src v_src = Some m_src0)
+      (SIMADDR: Val.inject sm0.(inj) addr_src addr_tgt)
+      (SIMV: Val.inject sm0.(inj) v_src v_tgt)
+  :
+    exists sm1,
+      (<<MSRC: sm1.(src) = m_src0>>)
+      /\ (<<MINJ: sm1.(inj) = sm0.(inj)>>)
+      /\ (<<STRTGT: Mem.storev chunk sm0.(tgt) addr_tgt v_tgt = Some sm1.(tgt)>>)
+      /\ (<<MWF: wf' sm1>>)
+      /\ (<<MLE: le' sm0 sm1>>)
+.
+Proof.
+  exploit Mem.storev_mapped_inject; try apply MWF; eauto. i; des.
+  unfold Mem.storev in STRSRC. des_ifs. inv SIMADDR. exploit store_mapped; eauto. i; des.
+  exists sm1. esplits; eauto. unfold Mem.storev.
+  hexploit (size_chunk_pos chunk); eauto. intro SZ.
+  assert(Ptrofs.unsigned i + delta = Ptrofs.unsigned (Ptrofs.add i (Ptrofs.repr delta))).
+  { rewrite <- Ptrofs.repr_unsigned with (i := i). rewrite Ptrofs.Ptrofs_add_repr.
+    rewrite Ptrofs.unsigned_repr; [|eapply Ptrofs.unsigned_range_2]. rewrite Ptrofs.unsigned_repr; eauto.
+    eapply Mem.mi_representable; eauto.
+    left. eapply Mem.perm_store_1; eauto. eapply Mem.perm_implies; [|eauto with mem]. eapply Mem.perm_cur_max.
+    eapply Mem.store_valid_access_3 in STRSRC. destruct STRSRC. eapply H1. omega.
+  }
+  rewrite <- H1. eauto.
+Qed.
+
+Lemma free_parallel
+      sm0 lo hi blk_src blk_tgt delta m_src0
+      (MWF: wf' sm0)
+      (FREESRC: Mem.free sm0.(src) blk_src lo hi = Some m_src0)
+      (SIMBLK: sm0.(inj) blk_src = Some (blk_tgt, delta))
+  :
+    exists sm1,
+      (<<MSRC: sm1.(src) = m_src0>>)
+      /\ (<<MINJ: sm1.(inj) = sm0.(inj)>>)
+      /\ (<<FREETGT: Mem.free sm0.(tgt) blk_tgt (lo + delta) (hi + delta) = Some sm1.(tgt)>>)
+      /\ (<<MWF: wf' sm1>>)
+      /\ (<<MLE: le' sm0 sm1>>)
+.
+Proof.
+  exploit Mem.free_parallel_inject; try apply MWF; eauto. i; des.
+  inv MWF.
+  eexists (mk _ _ _ _ _ _ _).
+  esplits; ss; eauto; cycle 1.
+  - econs; ss; eauto.
+    + eapply Mem.free_unchanged_on; eauto.
+      ii. apply SRCEXT in H2. red in H2. des. red in H2. clarify.
+    + eapply Mem.free_unchanged_on; eauto.
+      ii. apply TGTEXT in H2. red in H2. des. red in H2.
+      eapply H2; eauto. clear - FREESRC H1 H4.
+      apply Mem.free_range_perm in FREESRC. eauto with mem xomega.
+    + eapply frozen_refl.
+    + ii. eapply Mem.perm_free_3; eauto.
+    + ii. eapply Mem.perm_free_3; eauto.
+  - econs; ss; eauto.
+    + etransitivity; eauto. unfold src_private. ss. ii; des. esplits; eauto.
+      unfold valid_blocks in *. eauto with mem.
+    + etransitivity; eauto. unfold tgt_private. ss. ii; des. esplits; eauto.
+      { ii. eapply PR. eauto with mem. eauto with mem. }
+      unfold valid_blocks in *. eauto with mem.
+    + etransitivity; eauto. erewrite <- Mem.nextblock_free; eauto. xomega.
+    + etransitivity; eauto. erewrite <- Mem.nextblock_free; eauto. xomega.
+Qed.
+
+Lemma free_left
+      sm0 lo hi blk_src blk_tgt delta m_src0
+      (MWF: wf' sm0)
+      (FREESRC: Mem.free sm0.(src) blk_src lo hi = Some m_src0)
+      (SIMBLK: sm0.(inj) blk_src = Some (blk_tgt, delta))
+  :
+    exists sm1,
+      (<<MSRC: sm1.(src) = m_src0>>)
+      /\ (<<MTGT: sm1.(tgt) = sm0.(tgt)>>)
+      /\ (<<MINJ: sm1.(inj) = sm0.(inj)>>)
+      /\ (<<MWF: wf' sm1>>)
+      /\ (<<MLE: le' sm0 sm1>>)
+.
+Proof.
+  exploit Mem.free_left_inject; try apply MWF; eauto. i; des.
+  inv MWF.
+  eexists (mk _ _ _ _ _ _ _).
+  esplits; ss; eauto; cycle 1.
+  - econs; ss; eauto.
+    + eapply Mem.free_unchanged_on; eauto.
+      ii. apply SRCEXT in H1. red in H1. des. red in H1. clarify.
+    + eapply Mem.unchanged_on_refl.
+    + eapply frozen_refl.
+    + ii. eapply Mem.perm_free_3; eauto.
+  - econs; ss; eauto.
+    + etransitivity; eauto. unfold src_private. ss. ii; des. esplits; eauto.
+      unfold valid_blocks in *. eauto with mem.
+    + etransitivity; eauto. unfold tgt_private. ss. ii; des. esplits; eauto.
+      { ii. eapply PR. eauto with mem. eauto with mem. }
+    + etransitivity; eauto. erewrite <- Mem.nextblock_free; eauto. xomega.
+Qed.
+
+Lemma free_right
+      sm0 lo hi blk_tgt m_tgt0
+      (MWF: wf' sm0)
+      (FREETGT: Mem.free sm0.(tgt) blk_tgt lo hi = Some m_tgt0)
+      (PRIVTGT: forall ofs (BDD: lo <= ofs < hi), sm0.(tgt_private) blk_tgt ofs)
+      (EXTTGT: forall ofs : Z, lo <= ofs < hi -> ~ tgt_external sm0 blk_tgt ofs)
+  :
+    exists sm1,
+      (<<MSRC: sm1.(src) = sm0.(src)>>)
+      /\ (<<MTGT: sm1.(tgt) = m_tgt0>>)
+      /\ (<<MINJ: sm1.(inj) = sm0.(inj)>>)
+      /\ (<<MWF: wf' sm1>>)
+      /\ (<<MLE: le' sm0 sm1>>)
+.
+Proof.
+  exploit Mem.free_right_inject; try apply MWF; eauto.
+  { ii. eapply PRIVTGT in H1. red in H1. des. red in H1. eapply H1; eauto.
+    replace (ofs + delta - delta) with ofs by omega. eauto with mem.
+  }
+  i; des.
+  inv MWF.
+  eexists (mk _ _ _ _ _ _ _).
+  esplits; ss; eauto; cycle 1.
+  - econs; ss; eauto.
+    + eapply Mem.unchanged_on_refl.
+    + eapply Mem.free_unchanged_on; eauto.
+    + eapply frozen_refl.
+    + ii. eapply Mem.perm_free_3; eauto.
+  - econs; ss; eauto.
+    + etransitivity; eauto. unfold tgt_private. ss. ii; des. esplits; eauto.
+      unfold valid_blocks in *. eauto with mem.
+    + etransitivity; eauto. erewrite <- Mem.nextblock_free; eauto. xomega.
+Qed.
+
+Lemma alloc_parallel
+      sm0 lo_src hi_src lo_tgt hi_tgt blk_src m_src0
+      (MWF: wf' sm0)
+      (ALCSRC: Mem.alloc sm0.(src) lo_src hi_src = (m_src0, blk_src))
+      (LO: lo_tgt <= lo_src)
+      (HI: hi_src <= hi_tgt)
+  :
+    exists sm1 blk_tgt ,
+      (<<MSRC: sm1.(src) = m_src0>>)
+      /\ (<<ALCTGT: Mem.alloc sm0.(tgt) lo_tgt hi_tgt = (sm1.(tgt), blk_tgt)>>)
+      /\ (<<INJ: sm1.(inj) blk_src = Some (blk_tgt, 0) /\ forall b, b <> blk_src -> sm1.(inj) b = sm0.(inj) b>>)
+      /\ (<<MWF: wf' sm1>>)
+      /\ (<<MLE: le' sm0 sm1>>)
+.
+Proof.
+  exploit Mem.alloc_parallel_inject; try apply MWF; eauto. i; des.
+  inv MWF.
+  eexists (mk _ _ f' _ _ _ _). exists b2.
+  esplits; ss; eauto; cycle 1.
+  - econs; ss; eauto.
+    + eapply Mem.alloc_unchanged_on; eauto.
+    + eapply Mem.alloc_unchanged_on; eauto.
+    + econs. ii. des.
+      destruct (eq_block b_src blk_src).
+      * subst. rewrite H2 in NEW0. clarify.
+        eapply Mem.alloc_result in ALCSRC. rewrite ALCSRC.
+        eapply Mem.alloc_result in H. rewrite H. esplits; eauto.
+      * rewrite H3 in NEW0; eauto. clarify.
+    + ii. eapply Mem.perm_alloc_4; eauto.
+      ii. subst b. eapply Mem.fresh_block_alloc; try eapply ALCSRC; eauto.
+    + ii. eapply Mem.perm_alloc_4; eauto.
+      ii. subst b. eapply Mem.fresh_block_alloc; eauto.
+  - econs; ss; eauto.
+    + etransitivity; eauto. unfold src_private. ss. ii; des. esplits; eauto.
+      { destruct (eq_block x0 blk_src).
+        - subst x0. exfalso. eapply Mem.fresh_block_alloc; try eapply ALCSRC; eauto.
+        - r. rewrite H3; eauto. }
+      unfold valid_blocks in *. eauto with mem.
+    + etransitivity; eauto. unfold tgt_private. ss. ii; des. esplits; eauto.
+      { ii. destruct (eq_block b0 blk_src).
+        - subst b0. clarify. eapply Mem.fresh_block_alloc; eauto.
+        - eapply PR. rewrite <- H3; eauto. eauto with mem. }
+      unfold valid_blocks in *. eauto with mem.
+    + etransitivity; eauto. eapply Mem.nextblock_alloc in ALCSRC. rewrite ALCSRC. xomega.
+    + etransitivity; eauto. eapply Mem.nextblock_alloc in H. rewrite H. xomega.
+Qed.
+
+End ORIGINALS.
+
+Record mcompat (sm0: t') (m_src0 m_tgt0: mem) (F: meminj): Prop := mkmcompat {
+  mcompat_src: sm0.(src) = m_src0;
+  mcompat_tgt: sm0.(tgt) = m_tgt0;
+  mcompat_inj: sm0.(inj) = F;
+}.
+
+End MEMINJ.
+
+Hint Unfold valid_blocks.
+Hint Unfold src_private tgt_private.
+
+Ltac compat_tac := ss; econs; eauto; try congruence.
+
+Ltac spl := esplits; [|reflexivity].
+Ltac spl_approx sm :=
+  eexists (mk _ _ _ sm.(src_external) sm.(tgt_external) sm.(src_parent_nb) sm.(tgt_parent_nb)); splits; eauto.
+Ltac spl_exact sm :=
+  exists sm; splits; [|try etransitivity; eauto; try reflexivity; eauto].
